arithmetic/coq/Verif_add_with_carry.v
@@ -1,0 +1,49 @@
+Require Import VST.floyd.proofauto.
+Require Import VST.floyd.library.
+
+Require Import Didactica.arithmetic.
+Require Import Didactica.Add.
+Require Import Didactica.number.
+
+Lemma body_add_with_carry : semax_body Vprog Gprog f_add_with_carry add_with_carry_spec.
+Proof.
+  start_function.
+  unfold digit_bound in *.
+  forward. deadvars!. normalize.
+(*
+  replace
+    (Int64.repr (left_digit + Z.b2z carry_in))
+  with
+    (Int64.repr
+      (Z.modulo
+        (left_digit + Z.b2z carry_in)
+        Int64.max_unsigned)).
+  admit.
+  Search (@eq int _ _).
+  Check eq.
+
+  unfold Int64.repr.
+  replace
+    (Int64.Z_mod_modulus
+      ((left_digit + Z.b2z carry_in) mod Int64.max_unsigned))
+  with
+    (((left_digit + Z.b2z carry_in) mod Int64.max_unsigned) mod Int64.max_unsigned).
+  reflexiv
+  rewrite Int64.Z_mod_modulus_eq.
+  Search Int64.Z_mod_modulus.
+
+  Search Int64.repr.
+  forward. normalize.
+  forward.
+  replace
+    (Int64.ltu
+      (Int64.repr (left_digit + Z.b2z carry_in))
+      (Int64.repr (Z.b2z carry_in)))
+  with
+    (Z.ltb
+      (Z.modulo (Z.b2z carry_in + left_digit) Int64.max_unsigned)
+      (Z.b2z carry_in)). admit.
+  normalize.
+  entailer!. forward.
+  *)
+Admitted.
